

$$\begin{bmatrix} \phi_{t+1} \\ w_{t+1} \end{bmatrix} = \begin{bmatrix} 1 & 3 \\ -2 & 1 \end{bmatrix} \begin{bmatrix} \phi_t \\ w_t \end{bmatrix}$$

$$l_i(\underbrace{\phi, w}_{\theta}) = \frac{1}{2} (y_i - \underbrace{m_i}_{m_i}^T \theta)^2$$

$$\begin{bmatrix} \phi_t \\ w_t \end{bmatrix} = \theta_{t+1} = A \theta_t + \xi_t$$

$$\left(\underbrace{\begin{bmatrix} m_i^{\phi} \\ m_i^w \end{bmatrix}}_{m_i}, y_i \right)$$

$$\underline{y}_i = \underline{\underline{m_i}}^T \underline{\underline{\theta_t}}$$

$$= m_{\phi,i}^T \phi_t + m_{w,i}^T w_t$$